Port a proof from nik_lowstar in order to remove an admit

src/arch/x64/Views.fst
@@ -104,31 +104,52 @@ let get64_def (s:Seq.lseq U8.t 8) =
     (U8.v (Seq.index s 7))    
   )
 
+private
+abstract
+let get64_def_alt (s:Seq.lseq U8.t 8) : GTot UInt64.t =
+  let open FStar.Mul in
+  let s0 = Seq.slice s 0 4 in
+  let u0 = get32_def s0 in
+  let s1 = Seq.slice s 4 8 in
+  let u1 = get32_def s1 in
+  UInt64.uint_to_t (UInt32.v u0 +
+                    UInt32.v u1 * 0x100000000)
+
+private
+let get64_def_alt_equiv (s:Seq.lseq U8.t 8)
+  : Lemma (get64_def s == get64_def_alt s)
+  = ()
+
 let put64_def (a:UInt64.t) : GTot (Seq.lseq U8.t 8) =
-  let s = Seq.create 8 (U8.uint_to_t 0) in
-  let x = UInt64.v a in
-  let s = Seq.upd s 0 (U8.uint_to_t (x % 0x100)) in
-  let x = x `op_Division` 0x100 in
-  let s = Seq.upd s 1 (U8.uint_to_t (x % 0x100)) in
-  let x = x `op_Division` 0x100 in
-  let s = Seq.upd s 2 (U8.uint_to_t (x % 0x100)) in
-  let x = x `op_Division` 0x100 in
-  let s = Seq.upd s 3 (U8.uint_to_t (x % 0x100)) in
-  let x = x `op_Division` 0x100 in
-  let s = Seq.upd s 4 (U8.uint_to_t (x % 0x100)) in
-  let x = x `op_Division` 0x100 in
-  let s = Seq.upd s 5 (U8.uint_to_t (x % 0x100)) in
-  let x = x `op_Division` 0x100 in
-  let s = Seq.upd s 6 (U8.uint_to_t (x % 0x100)) in
-  let x = x `op_Division` 0x100 in
-  let s = Seq.upd s 7 (U8.uint_to_t (x % 0x100)) in
-  s
+  let u0 = UInt32.uint_to_t (UInt64.v a % 0x100000000) in
+  let u1 = UInt32.uint_to_t ((UInt64.v a / 0x100000000) % 0x100000000) in
+  let s0 = put32_def u0 in
+  let s1 = put32_def u1 in
+  Seq.append s0 s1
+
+private
+let inverses64_def_aux (x:UInt64.t)
+  : Lemma (get64_def (put64_def x) == x)
+  = ()
+
+private
+let inverses64_def_aux' (x:Seq.lseq U8.t 8)
+  : Lemma (put64_def (get64_def x) `Seq.equal` x)
+  = reveal_opaque get32_def;
+    reveal_opaque put32_def;
+    inverses32();
+    get64_def_alt_equiv x;
+    get64_def_alt_equiv (put64_def (get64_def x));
+    inverses64_def_aux (get64_def x)
 
 let get64 = make_opaque get64_def
-let put64  = make_opaque put64_def
+let put64 = make_opaque put64_def
 
-//TODO
-let inverses64 (u:unit) : Lemma (inverses get64 put64) = admit()
+let inverses64 (u:unit) : Lemma (inverses get64 put64) =
+  reveal_opaque get64_def;
+  reveal_opaque put64_def;
+  Classical.forall_intro inverses64_def_aux;
+  Classical.forall_intro inverses64_def_aux'
 
 let view64 = inverses64 (); View 8 get64 put64
 
